Loop$ improvements: (1) ignorable is implicit in lambda$; (2) locals/globals switch in fancy loops; (3) :doc loop$; Special Conjectures for guards improved with (4) member-equal instead of mempos and with (5) warrant hypotheses,
Although J and I have lots of discussion about the design of these
loop$ improvements, implementation work for (1) through (4) were
essentially J's work and for (5) was essentially mine.

(1) Loop$ bodies continue to generate lambda$ expressions.  Formerly,
an ignorable declaration for the lambda$ formals was generated for
these lambda$ expressions.  Now they are not; instead, translation of
lambda$ to a quoted lambda is what generates the ignorable
declaration.  The benefit is that one no longer sees distracting
ignorable declarations in untranslated output arising from loops.

(2) Fancy loops continue to generate lambda$ expressions with two
arguments, representing loop variables and "global" variables not
bound by the loop variables.  Formerly the lambda$ parameter list was
(locals globals); those have been switched and renamed, resulting in
(LOOP$-GVARS LOOP$-IVARS), which is more intuitive (especially given
other aspects of loop$ translation).

(3) Formerly, :doc loop$ was little more than a stub.  That
documentation is now quite extensive.

(4) The so-called "Special Conjectures" are guard proof obligations to
support the use of Common Lisp loop to execute loop$ expressions in
function bodies during top-level evaluation.  These existed before;
but now, hypotheses about member-equal replace hypotheses about
mempos.  The new book books/projects/apply/mempos.lisp can support
useful reasoning about mempos, including fancy loops.

(5) Formerly it was necessary to specify warrant hypotheses in guards,
which defeated evaluation during proofs.  Consider the following
example, where at the end we attempt a proof using evaluation, by
disabling a definition to prevent proof by rewriting.

(include-book "projects/apply/top" :dir :system)
(defun$ double (n)
  (declare (xargs :guard (integerp n)))
  (+ n n))
(defun sum-doubles (lst)
  (declare (xargs :guard (and (warrant double) ; to be removed
                              (integer-listp lst))))
  (loop$ for x of-type integer in lst sum (double x)))
; Fails:
(thm (implies (warrant double)
              (equal (sum-doubles '(1 2 3)) 12))
     :hints (("Goal" :in-theory (disable (:d sum-doubles)))))

The thm fails because the attempt to execute sum-doubles fails with an
error: the guard cannot be evaluated during the proof.  (Remarks.  (a)
Warrants are constrained functions and need attachments to evaluate,
which aren't available during proofs.  (b) Perhaps guard evaluation
failure shouldn't defeat execution but should just punt to *1*
evaluation.  That may be future work.)  Before this change, the
hypothesis (warrant double) was necessary for guard verification of
sum-doubles.  Now it is no longer needed, because Special Conjectures
include warrant hypotheses.

Note: In addition to changes (1) through (5) there are a few tweaks,
for example in error messages involving ignore and ignorable
declarations.

In addition to running a clean regression-everything, I also built a
#+acl2-devel executable and went through the process described in a
comment in the source definition of *system-verify-guards-alist*.

books/system/doc/acl2-doc.lisp
@@ -5256,9 +5256,13 @@ and @(tsee include-book)"
   <li>@(tsee lambda$) expression -- an ACL2 macro that allows you to enter
       quoted well-formed @('LAMBDA') objects into your terms by typing
       untranslated expressions that resemble lambda expressions.  The
-      @('lambda$') expression @('(lambda$ (x) (+ 1 x))') translates into the
-      quoted @('LAMBDA') object @(''(LAMBDA (X) (BINARY-+ '1 X))').  See also
-      @(see lambda) for some clarifications.</li>
+      @('lambda$') expression @('(lambda$ (x) (+ 1 x))') essentially translates
+      into the quoted @('LAMBDA') object @(''(LAMBDA (X) (BINARY-+ '1 X))').
+      We say ``essentially'' because @('lambda$') always inserts a
+      @('(DECLARE (IGNORABLE v1 ... vn))') listing every formal and tags the
+      body with a @(tsee RETURN-LAST) form that indicates it came from a
+      translated @('lambda$'). See also @(see lambda) for some
+      clarifications.</li>
 
   <li>@(tsee scion) -- a function that is ancestrally dependent on @('apply$'),
       sometimes (perhaps misleadingly) called a ``mapping function.''  An
@@ -47375,15 +47379,20 @@ tables in the current Hons Space."
   (collect (lambda$ (x) (+ 1 x)) lst)
   })
 
-  <p>That @('lambda$') expression translate to the quoted well-formed
-  @('LAMBDA') object</p>
+  <p>That @('lambda$') expression essentially translates to the quoted
+  well-formed @('LAMBDA') object</p>
 
   @({
   '(LAMBDA (X) (BINARY-+ '1 X))
   })
 
   <p>Note that the body is fully translated, unlike its appearance in the
-  @('lambda$') expression.</p>
+  @('lambda$') expression.  We say ``essentially'' because @('lambda$') always
+  add a @('(DECLARE (IGNORABLE v1 ... vn))') that includes every formal.  In
+  addition, except when translating in theorems, @('lambda$') tags the
+  translated body with a @(tsee RETURN-LAST) expression to indicate it came
+  from a @('lambda$').  Despite these differences, the meaning of the
+  translated @('lambda$') is the simple quoted @('LAMBDA') object shown.</p>
 
   <p>@('Lambda$') expressions never appear in a fully translated term.  All the
   @('lambda$') objects will have been translated into quoted @('LAMBDA')
@@ -47435,7 +47444,6 @@ tables in the current Hons Space."
   (lambda$ (n lst str)
            (declare (type integer n)
                     (type string str)
-                    (ignore str)
                     (xargs :guard (and (posp n)
                                        (true-listp lst)
                                        (&lt; (- n 1) (length lst)))))
@@ -47451,17 +47459,16 @@ tables in the current Hons Space."
   returning 1 value.  @('Body') must satisfy the same restrictions one would
   expect in a non-recursive @(tsee defun) event with the same formals,
   declarations and body.  In particular, @('body') should contain no free
-  variables other than those listed in @('vars'), must not use freely any
-  variable declared @('IGNORE')d and must use every other variable in @('vars')
-  except, possibly, variables listed as @('IGNORABLE').  @('Lambda$') expands
-  to a well-formed quoted @('LAMBDA') object or else causes a translate-time
-  error.</p>
+  variables other than those listed in @('vars').  @('Lambda$') always adds a
+  declaration that every formal is ignorable and, hence, we prohibit you from
+  adding @('ignore') or @('ignorable') declarations in the @('lambda$')
+  expression itself.  @('Lambda$') expands to a well-formed quoted @('LAMBDA')
+  object or else causes a translate-time error.</p>
 
-  <p>The allowed @('DECLARE') forms in @('lambda$') are @('type'), @('ignore'),
-  @('ignorable') and @('xargs').  Furthermore, the only @(tsee xargs) keywords
-  allowed are @(':guard') and @(':split-types').  The other @('XARGS')
-  keywords, such as @(':measure'), @(':hints') or @(':guard-hints'), play no
-  role.</p>
+  <p>The allowed @('DECLARE') forms in @('lambda$') are @('type') and
+  @('xargs').  Furthermore, the only @(tsee xargs) keywords allowed are
+  @(':guard') and @(':split-types').  The other @('XARGS') keywords, such as
+  @(':measure'), @(':hints') or @(':guard-hints'), play no role.</p>
 
   <h3>About Guard Verification of Lambda Objects</h3>
 
@@ -51487,27 +51494,683 @@ tables in the current Hons Space."
 (defxdoc loop$
   :parents (acl2-built-ins programming)
   :short "Iteration with an analogue of the Common Lisp @('loop') macro"
-  :long "<p>This documentation is currently little more than a stub.  We expect
- to provide more complete documentation for @('loop$') before the next ACL2
- release.  In brief: @('Loop$') is an ACL2 version of the Common Lisp @('loop')
- macro.</p>
+  :long "<p>@('Loop$') is the ACL2 analogue of the Common Lisp's iteration
+  primitive, @('loop').  This documentation assumes the reader has at least a
+  passing familiarity with @('loop').</p>
 
- <p>In the meantime, you can see @(see community-books)
- @('books/system/tests/loop-tests.lisp') and
- @('books/system/tests/apply-in-proofs.lisp') for numerous examples.</p>
+  <p><b>Warning:</b> @('Loop$') implements only a small part of the
+  functionality of @('loop').  Aside from the simple fact that @('loop$')
+  allows a small subset of the syntax of @('loop'), the main restriction is
+  that the subexpressions of the @('loop$') statement that are evaluated
+  repeatedly must be @(see tame)!  These expressions include the @('until')
+  test, the @('when') test, and the @('loop$') body.  For example, this means
+  that @('loop$') does not allow iterations involving @(tsee state) or @(see
+  stobj)s.</p>
 
- <p>When a term is a call of @('loop$'), is to be evaluated at the top level or
- during a proof, and is a ground term (has no free variables), then that term
- is translated to a call involving so-called ``loop$ scions'' before it is
- evaluated.  For example, after evaluating @('(defun$ f (x) (cons x x))'), such
- an attempt to evaluate @('(loop$ for x in '(a b c) collect (f x))')
- essentially becomes an evaluation of the following call of the loop$ scion,
- @('collect$').</p>
+  <h3>Informal Introduction</h3>
 
- @({
- (COLLECT$ '(LAMBDA (X) (F X))
-           '(A B C))
- })")
+  <p>ACL2's @('loop$') is considerably more restricted than Common Lisp's but
+  when an ACL2 @('loop$') statement is translated without error it has the same
+  meaning as the corresponding Common Lisp @('loop').  (Note: @('loop$') allows
+  @(':guard') declarations in certain places and these are ignored by Common
+  Lisp.)</p>
+
+  <p>We give some examples of legal @('loop$') statements below.  We deal with
+  guards and guard verification later in this topic.</p>
+
+  @({
+  ACL2 !>(loop$ for x in '(1 2 3) sum (* x x))
+  14
+  ACL2 !>(loop$ for x in '(1 2 3) collect (* x x))
+  (1 4 9)
+  ACL2 !>(loop$ for x on '(1 2 3) collect x)
+  ((1 2 3) (2 3) (3))
+  ACL2 !>(loop$ for x from -10 to 10 by 2 collect x)
+  (-10 -8 -6 -4 -2 0 2 4 6 8 10)
+  ACL2 !>(loop$ for i from 1 to 10
+                as  x in '(a b c d e f g)
+                collect (cons i x))
+  ((1 . A)
+   (2 . B)
+   (3 . C)
+   (4 . D)
+   (5 . E)
+   (6 . F)
+   (7 . G))
+  ACL2 !>(loop$ for i from 1 to 10
+                as  x in '(a b c d e f g)
+                until (> i 6)
+                collect (cons i x))
+  ((1 . A)
+   (2 . B)
+   (3 . C)
+   (4 . D)
+   (5 . E)
+   (6 . F))
+  ACL2 !>(loop$ for i from 1 to 10
+                as  x in '(a b c d e f g)
+                until (> i 6)
+                when (evenp i)
+                collect (cons i x))
+  ((2 . B) (4 . D) (6 . F))
+  })
+
+  <p>@('Loop$') statements execute fastest when they are guard verified.  But
+  the @('until'), @('when'), and @('loop$') body raise interesting guard
+  verification problems because they are executed for many different values of
+  the iteration variables.  It may be necessary to provide type information or
+  even stronger invariants to verify their guards.  We now provide a few
+  examples illustrating the handling of guards in @('loop$').</p>
+
+  <p>The first example below is an acceptable @('loop$') statement but cannot
+  be guard verified, as would be necessary if it appeared in a @(tsee defun)
+  that was to be guard verified.  The problem is that @('(+ 1 x)') requires
+  @('x') to be numeric and, in general, we don't know anything about the value
+  of @('x') here.  (Actually, because the target range is just a constant
+  below, we could deduce information about each value @('x') takes on, but we
+  don't.)  The second example can be guard verified and has the advantage of
+  being standard Common Lisp so compilers might optimize the handing of @('(+ 1
+  x)').  The third example can also be guard verified but since the @(':guard')
+  derective used here is ignored by Common Lisp it does not inform the
+  compiler, so this example might execute more slowly than the previous one.
+  The last example shows the syntax and use of the ACL2-specific addition to
+  @('loop$'): the @(':guard') directive protecting, in this case, the
+  @('loop$') body.  @(':Guard') is useful when you wish to add more guard
+  information than can be expressed with the Common Lisp @('of-type')
+  directive.  The @('of-type') and @(':guard') directives are conjoined to form
+  the actual guard protecting the @('loop$') body.</p>
+
+  @({
+  ACL2 !>(loop$ for x in '(1 2 3) collect (+ 1 x))
+  (2 3 4)
+  ACL2 !>(loop$ for x of-type integer in '(1 2 3) collect (+ 1 x))
+  (2 3 4)
+  ACL2 !>(loop$ for x in '(1 2 3) collect :guard (integerp x) (+ 1 x))
+  (2 3 4)
+  ACL2 !>(let ((max 10))
+          (loop$ for x of-type integer in '(1 2 3) 
+                 collect :guard (and (integerp max) (< x max)) (- max x)))
+  (9 8 7)
+  })
+
+  <p>The guard on the @('(- max x)') above is @('(and (integerp x) (integerp
+  max) (< x max))') and the compiler is informed that @('x') is an integer by
+  the @('of-type').</p>
+
+  <p>As of ACL2 Version 8.2, the only allowed iteration clauses are @('in'),
+  where the variable ranges over the elements of the given true list, @('on'),
+  where the variable ranges over the tails of the given true-list, and
+  @('from/to/by') where the variable ranges over the integers between two
+  bounds, stepping by a positive integer increment (or by 1 if no @('by')
+  clause is provided.)</p>
+
+  <p>You may have as many iteration clauses as you wish, connected with
+  @('as').  Each must introduce a unique iteration variable and that variable
+  may be optionally followed by an @('of-type') @(tsee type-spec)
+  specification.  @('Of-type') is a Common Lisp feature that allows the
+  compiler to optimize operations on the variable in question.  An
+  example is</p>
+
+  @({
+  (loop$ for v of-type (and integer (not (satisfies zerop)))
+               from 1 to 100
+         sum (/ 1 v))
+  })
+
+  <p>After all of the iteration clauses, you may have a termination test,
+  signaled by @('until'), and/or a conditional test signaled by @('when').  If
+  both are provided, the @('until') test must come first.  Iteration stops when
+  the @('until') test is satisfied.  The conditional test determines whether
+  the loop body is executed for the current value of the iteration
+  variables.</p>
+
+  <p>Between the @('until') symbol and the expression to be tested, and between
+  the @('when') symbol and its expression, you may include a @(':guard')
+  clause.  This is useful if guard verification requires an invariant relating
+  multiple iteration variables.  And example of a guarded @('until') clause is</p>
+
+  @({
+  (loop$ for u in lst1 as v in lst2
+         until :guard (invariantp u v) (test u v)
+         collect (body u v))
+  })
+
+  <p>ACL2 Version 8.2 supports only four operators, @('sum'), @('collect'),
+  @('always') and @('append').  We anticipate adding other Common Lisp
+  operators eventually.</p>
+
+  <p>Between the operator, e.g., @('sum') or @('collect'), and the
+  @('loop$') body you may include a @(':guard') clause as in</p>
+
+  @({
+  (loop$ for u in lst1 as v in lst2
+         collect :guard (invariantp u v) (body u v))
+  })
+
+  <p>This is sometimes necessary in the verification of the guards for the
+  @('loop$') body because Common Lisp's @('of-type') clauses do not permit you
+  to relate one variable to another.</p>
+
+  <h3>General Form</h3>
+
+  <p>The syntax of Common Lisp @('loop') statements is extremely complicated.
+  Rather than try to write the abstract syntax of ACL2's @('loop$') statements
+  in the same formal style, we take a different approach, which is workable
+  because @('loop$') allows fewer options.</p>
+
+  <p>First we introduce the syntax of a ``target clause,'' a ``type-spec,'' and
+  the ``operators.''  Then we describe the most elaborate form of a @('loop$')
+  statement in terms of these elements and ordinary ACL2 terms.  Every legal
+  @('loop$') statement can be produced by omitting certain optional elements
+  from the most elaborate @('loop$') form.  So we conclude the syntactic
+  description of @('loop$') by listing the elements that can be omitted.</p>
+
+  <p>A <i>target clause</i> has one of four forms</p>
+
+  <ul>
+  <li>@('IN') <i>list-expr</i></li>
+
+  <li>@('ON') <i>list-expr</i></li>
+
+  <li>@('FROM') <i>lo-expr</i> @('TO') <i>hi-expr</i></li>
+
+  <li>@('FROM') <i>lo-expr</i> @('TO') <i>hi-expr</i> @('BY') <i>step-expr</i></li>
+
+  </ul>
+
+  <p>where <i>list-expr</i> is a term (which is expected to evaluate to a true
+  list), <i>lo-expr</i> and <i>hi-expr</i> are terms (which are expected to
+  evaluate to integers), and <i>step-expr</i> is a term (which is expected to
+  evaluate to a positive integer).</p>
+
+  <p>The legal <i>type-specs</i> are listed in @(tsee type-spec).</p>
+
+  <p>The legal <i>operators</i> are @('SUM'), @('COLLECT'), @('ALWAYS'), and
+  @('APPEND').</p>
+
+  <p>The most elaborate @('loop$') statement is of the form</p>
+
+  &nbsp; &nbsp; &nbsp; &nbsp; @('(LOOP$ FOR ')<i>v1</i>@(' OF-TYPE ')<i>spec1
+  target1</i><br/> &nbsp; &nbsp; &nbsp; &nbsp; &nbsp; &nbsp; &nbsp; &nbsp;
+  &nbsp; &nbsp; &nbsp; &nbsp; @('AS ') &nbsp; <i>v2</i>@(' OF-TYPE ')<i>spec2
+  target2</i><br/> &nbsp; &nbsp; &nbsp; &nbsp; &nbsp; &nbsp; &nbsp; &nbsp;
+  &nbsp; &nbsp; &nbsp; &nbsp; ...<br/> &nbsp; &nbsp; &nbsp; &nbsp; &nbsp;
+  &nbsp; &nbsp; &nbsp; &nbsp; &nbsp; &nbsp; &nbsp; @('AS ') &nbsp; <i>vn</i>@('
+  OF-TYPE ')<i>specn targetn</i><br/> &nbsp; &nbsp; &nbsp; &nbsp; &nbsp; &nbsp;
+  &nbsp; &nbsp; &nbsp; &nbsp; &nbsp; &nbsp; @('UNTIL :GUARD ')<i>guard1
+  until-expr</i><br/> &nbsp; &nbsp; &nbsp; &nbsp; &nbsp; &nbsp; &nbsp; &nbsp;
+  &nbsp; &nbsp; &nbsp; &nbsp; @('WHEN ') &nbsp; @(':GUARD ')<i>guard2
+  when-expr</i>&nbsp; &nbsp; &nbsp; &nbsp; ; Note the @('ALWAYS') Exception
+  below!<br/> &nbsp; &nbsp; &nbsp; &nbsp; &nbsp; &nbsp; &nbsp; &nbsp; &nbsp;
+  &nbsp; &nbsp; &nbsp; <i>op</i>@(' :GUARD ')<i>guard3
+  body-expr</i>@(')')<br/>
+
+
+  <p>where each <i>vi</i> &nbsp; is a legal variable symbol and they are all
+  distinct, each <i>type-speci</i> &nbsp; is a @(tsee type-spec), each
+  <i>targeti</i> &nbsp; is a target clause, each <i>guardi</i>,
+  <i>until-expr</i>, and <i>when-expr</i> &nbsp; is a term, <i>op</i> &nbsp; is
+  an operator, and <i>body-expr</i> &nbsp; is a term.  Furthermore,
+  <i>until-expr</i>, <i>when-expr</i>, and <i>body-expr</i> &nbsp; must be
+  @(see tame)!</p>
+
+  <p><i>The @('ALWAYS') Exception:</i> Common Lisp prohibits loops with both a
+  @('WHEN') clause and an @('ALWAYS') operator.  If you are tempted to use
+  @('WHEN') <i>p</i> with @('ALWAYS') <i>q</i> we recommend you write
+  @('ALWAYS') @('(implies ')<i>p q</i>@(')').</p>
+
+  <p>The following elements may be omitted.</p>
+
+  <ul>
+  <li>any line beginning with @('AS'), @('UNTIL') or @('WHEN'),</li>
+
+  <li>any @('OF-TYPE') <i>speci</i>, and</li>
+
+  <li>any @(':GUARD') <i>guardi</i>.</li>
+
+  </ul>
+
+  <p>We give names to certain classes of the syntactic entities above.  The
+  <i>v1</i>, ..., <i>vn</i> are called the <i>iteration variables</i>.  The
+  <i>spec1</i>, ..., <i>specn</i> are called <i>type specs</i>, each corresponds to
+  a certain iteration variable, and each gives rise to a <i>type term</i> about
+  its variable in the sense that ``@('X OF-TYPE (SATISFIES NATP)')'' gives rise
+  to the type term @('(NATP X)') and ``@('I OF-TYPE INTEGER')'' gives rise to
+  the type term @('(INTEGERP I)').  The terms involved in the target
+  expressions, e.g., the <i>list-expr</i> in ``@('IN') <i>list-expr</i>'' and
+  ``@('ON') <i>list-expr</i>'' and the <i>lo-expr</i>, <i>hi-expr</i> and
+  optional <i>step-expr</i> in the ``@('FROM') <i>lo-expr</i> @('TO')
+  <i>hi-expr</i> @('BY') <i>step-expr</i>'' targets are called <i>target
+  terms</i>.  Finally, the <i>until-expr</i>, <i>when-expr</i>, and
+  <i>body-expr</i> are called <i>iterative forms</i>.</p>
+
+  <p>We distinguish the target terms from the iterative forms because they are
+  handled very differently at evaluation time.  When a @('loop$') is evaluated,
+  the target terms are evaluated just once.  But the iterative forms are
+  evaluated multiple times as the iteration variables range over the values of
+  the targets.</p>
+
+  <p>A @('loop$') statement with just one iteration variable and in which the
+  iterative forms mention no free variable other than the iteration variable
+  is called a <i>simple @('loop$')</i>.  An example of a simple loop is</p>
+
+  @({
+  (loop$ for x in lst when (evenp x) collect (+ 1 (sq x)))
+  })
+
+  <p>A @('loop$') statement called a <i>fancy @('loop$')</i> if it is not
+  simple.  Both of the following @('loop$')s are fancy.</p>
+
+  @({
+  (loop$ for x in xlst as y on ylst collect (expr x y))
+
+  (loop$ for x in xlst collect (expr x z))
+  })
+
+  <p>The first is fancy because it has two iteration variables.  The second is
+  fancy because the body freely uses the variable @('z') which is not the
+  iteration variable.</p>
+
+  <h3>Semantics</h3>
+
+  <p>@('Loop$') expressions are translated into calls of @(see scion)s, with
+  the @('until') and @('when') clauses translated into preprocessors of the
+  targets.  But which scions are used depend on whether the loop is simple or
+  fancy.  Recall that a fancy loop is one that has either or both of the
+  following characteristics: (a) there is one or more @('as') clauses,
+  and/or (b) one of the iterative forms (the @('until'), @('when') or loop body
+  expression) refers to variables other than an iteration variable.  If the
+  @('loop$') statement is simple, the simple scions are used; otherwise the
+  fancy scions are used.</p>
+
+  @({
+   loop$
+   syntax              simple          fancy
+   symbol              scion           scion
+   ______________________________________________
+   sum                 sum$            sum$+
+   collect             collect$        collect$+
+   always              always$         always$+
+   append              append$         append$+
+   until               until$          until$+
+   when                when$           when$+
+   })
+
+  <p>We deal with simple @('loop$')s first.</p>
+
+  <h4>Semantics of Simple Loop$s</h4>
+
+  <p>For example, the simple @('loop$')</p>
+  @({
+  (loop$ for x in lst collect (+ 1 (sq x)))
+  })
+  <p>translates to (a term equivalent to)</p>
+
+  @({
+  (collect$ (lambda$ (x)
+                     (declare (ignorable x))
+                     (+ 1 (sq x)))
+            lst).
+  })
+
+  <p><b>Note:</b> The actual translation is tagged with various markers that
+  play a role in evaluation but which are logically irrelevant and which are
+  removed during proof.  In this discussion we will not display the marked-up
+  translations but logically equivalent terms instead.  You can see the actual
+  translations for yourself with @(tsee trans).</p>
+
+  <p>In the translation the target term, @('lst'), appears as an ordinary
+  subterm of the translation.  But the iterative form, @('(+ 1 (sq x))'),
+  becomes the body of a @(tsee lambda$) expression, which means its translation
+  becomes a component of a quoted @('LAMBDA') object.  When the @('collect$')
+  is evaluated, the target term is evaluated once but the iterative form is
+  evaluated once for each element of the value of the target.</p>
+
+  <p>@('Until') and @('when') clauses are handled by preprocessing the target.
+  E.g.,</p>
+
+  @({
+  (loop$ for x in lst
+         until (> x 100)
+         when (evenp x)
+         collect (+ 1 (sq x)))
+  })
+
+  <p>becomes</p>
+
+  @({
+  (collect$ (lambda$ (x)
+                     (declare (ignorable x))
+                     (+ 1 (sq x)))
+            (when$ (lambda$ (x)
+                            (declare (ignorable x))
+                            (evenp x))
+                   (until$ (lambda$ (x)
+                                    (declare (ignorable x))
+                                    (> x 100))
+                           lst)))
+  })
+
+  <p>So from a logical perspective, the presence of an @('until') and/or
+  @('when') clause in a @('collect') iteration over @('lst') ``copies'' the
+  target value.  The @('until$') copies @('lst') until encountering the first
+  element on which its functional argument is true.  The @('when$') then copies
+  that (shortened?) target, keeping only the elements that satisfy its
+  functional argument.  Finally, the @('collect$') then applies its functional
+  argument and collects all the values.</p>
+
+  <p>@('ON') and @('FROM/TO/BY') targets are handled by listing all the
+  elements in the given target.  For example,</p>
+
+  @({
+  (loop$ for x on lst collect (expr x))
+  })
+
+  <p>which maps @('x') over successive tails of @('lst') and collects the value
+  of @('expr') has the logical meaning</p>
+
+  @({
+  (collect$ (lambda$ (x) (expr x))
+            (tails lst))
+  })
+
+  <p>where, for example, @('(tails '(1 2 3))') is @('((1 2 3) (2 3) (3))').</p>
+
+  <p>Spiritually similarly,</p>
+  @({
+  (loop$ for i from 1 to max by step collect (expr x))
+  })
+
+  <p>becomes</p>
+
+  @({
+  (collect$ (lambda$ (x) (expr x))
+            (from-to-by 1 max step))
+  })
+
+  <p>where, for example, @('(from-to-by 1 10 2)') is @('(1 3 5 7 9)').</p>
+
+  <p>Similar translations are done for the other operators, e.g., @('sum') and
+  @('always').  The advantage of this translation style is that it allows
+  compositional reasoning.  We discuss this further below.</p>
+
+  <h4>Semantics of Fancy Loop$s</h4>
+
+  <p>An example of a fancy @('loop$') is</p>
+
+  @({
+  (loop$ for x in xlst as y in ylst collect (expr x y z))
+  })
+
+  <p>This loop exhibits both characteristics (a) and (b): it has an @('as')
+  clause and the variable @('z') appears in the loop body.  Either
+  characteristic is sufficient to classify the loop as fancy.  So fancy scions
+  are used.  Its semantic counterpart, i.e., its translation, is</p>
+
+  @({
+  (collect$+
+   (lambda$ (loop$-gvars loop$-ivars)
+            (declare (xargs :guard (and (true-listp loop$-gvars)
+                                        (equal (len loop$-gvars) 1)
+                                        (true-listp loop$-ivars)
+                                        (equal (len loop$-ivars) 2))))
+            (let ((z (car loop$-gvars))
+                  (x (car loop$-ivars))
+                  (y (car (cdr loop$-ivars))))
+              (declare (ignorable x y))
+              (expr x y z)))
+   (list z)
+   (loop$-as (list xlst ylst)))
+   })
+
+  <p>Before we show the definition of @('collect$+') note that the arguments
+  above to @('collect$+') are (i) a @('lambda$') expression that handles the
+  evaluation of the iterative form, in this case @('(expr x y z)'), where
+  @('x') and @('y') are iteration variables and @('z') is a ``global'' variable
+  not among the iteration variables; (ii) the list of values of the ``global''
+  variables, in this case the list containing @('z'); and (iii) a target list
+  constructed by @('loop$-as') from the various targets provided in the
+  @('loop$'), in this case @('xlst') and @('ylst'), supplying values for
+  iteration variables @('x') and @('y') respectively.  For example,
+  @('(loop$-as (list '(a b c d e) '(1 2 3)))') is @('((a 1) (b 2) (c 3))').
+  These tuples contain successive corresponding values of @('x') and
+  @('y').</p>
+
+  <p>The definition of @('collect$+') is essentially</p>
+  @({
+  (defun collect$+ (fn loop$-gvars lst)
+    (if (endp lst)
+        nil
+        (cons (apply$ fn (list loop$-gvars (car lst)))
+              (collect$+ fn loop$-gvars (cdr lst)))))
+  })
+
+  <p>We have omitted the guard and an @('MBE') form that makes it run more
+  efficiently.  All the fancy @('loop$') scions are defined analogously.</p>
+
+  <p>Inspection of the @('lambda$') expression above reveals that it takes a a
+  list of global variable values and a list of iteration variable values,
+  unpacks them with a @('let') that binds the global variables, here just
+  @('z'), to their values and binds the iteration variables, here @('x') and
+  @('y'), to the corresponding pair of values from the target, and then
+  evaluates the @('loop$') body, @('(expr x y z)').</p>
+
+  <p>The names of the formals for the @('lambda$') expressions generated by
+  @('loop$') statements are always @('loop$-gvars') and @('loop$-ivars'), for
+  ``@('loop$') global variables'' and ``@('loop$') iteration variables.''</p>
+
+  <p>@('Until') and @('when') clauses in a fancy @('loop$') are handled exactly
+  as they are in simple @('loop$')s, except that the fancy scions are used
+  since the target list is a list of tuples of iteration variable values and
+  the @('until') and @('when') forms may refer to global variables.</p>
+
+  <h4>Special Guard Conjectures for LOOP$</h4>
+
+  <p>All of the simple @('loop$') scions have the same guard, namely</p>
+
+  @({
+  (AND (APPLY$-GUARD FN '(NIL))
+       (TRUE-LISTP LST)),
+  })
+
+  <p>and all the fancy @('loop$') scions have the same guard, namely</p>
+
+  @({
+  (AND (APPLY$-GUARD FN '(NIL NIL))
+       (TRUE-LISTP LOOP$-GVARS)
+       (TRUE-LIST-LISTP LST)).
+  })
+
+  <p>In addition to the normal guard conjectures that would be generated by
+  calls of these scions, ACL2 generates some special guard conjectures because
+  the normal guard conjectures are insufficient to guarantee the error-free
+  execution of the corresponding Common Lisp @('loop') statements.</p>
+
+  <p>For example, the logical meaning of</p>
+
+  @({
+  (defun foo (lst)
+    (declare (xargs :guard (and (warrant expr) (foo-guardp lst))))
+    (loop$ for x of-type (satisfies spec) on lst sum (expr x)))
+  })
+
+  <p>is</p>
+
+  @({
+  (defun foo (lst)
+    (declare (xargs :guard (foo-guardp lst)))
+    (sum$ (lambda$ (x)
+                   (declare (type (satisfies spec) x))
+                   (expr x))
+          (tails lst))).
+  })
+
+  <p>Prior to the provision for special guards, the normal guard conjectures
+  generated for @('foo') would be</p>
+
+  @({
+  (and (implies (foo-guardp lst)                                 ; [1]
+                (apply$-guard
+                 (lambda$ (x)
+                   (declare (type (satisfies spec) x))
+                   (expr x))
+                 '(nil)))
+       (implies (foo-guardp lst)                                 ; [2]
+                (true-listp (tails lst)))
+       (implies (foo-guardp lst)                                 ; [3]
+                (true-listp lst))
+       (implies (spec x) (expr-guardp x)))                       ; [4]
+  })
+
+  <p>Conjectures [1] and [2] stem from the guard for @('sum$') and establish
+  that the guard for @('foo') implies that @('sum$') is passed a function
+  object of one argument and a true-list.  Conjecture [3] establishes the guard
+  of @('tails').  And conjecture [4] establishes that the guard on the
+  @('lambda$') implies the guard of its body.</p>
+
+  <p>But consider the @('loop') generated by the @('loop$') in the raw Lisp
+  definition of @('foo'),</p>
+
+  @({
+  (loop for x of-type (satisfies spec) on lst sum (expr x)).
+  })
+
+  <p>For this @('loop') to execute without error we need to know that [5] every
+  non-empty tail of @('lst') satisfies @('spec'), [6] that for every tail,
+  @('x'), of @('lst'), @('(expr x)') returns a number, and [7] that @('nil')
+  satisfies @('spec').  The last is somewhat surprising but inspection of
+  Common Lisp reveals that even though @('(expr x)') is never called on the
+  empty tail of @('lst'), implementations running with high safety settings
+  check that the empty list satisfies @('spec').</p>
+
+  <p>So when ACL2's guard verification process encounters a @('sum$') like that
+  in the logical @('defun') of @('foo'), it generates three additional guard
+  conjectures</p>
+
+  @({
+       (implies (and (foo-guardp lst)                            ; [5]
+                     (member-equal newv (tails lst)))
+                (spec newv))
+
+       (implies (and (foo-guardp lst)                            ; [6]
+                     (member-equal newv (tails lst)))
+                (acl2-numberp
+                 (apply$ (lambda$ (x)
+                           (declare (type (satisfies spec) x))
+                           (expr x))
+                         (list newv))))
+
+       (implies (foo-guardp lst)                                 ; [7]
+                (spec nil))
+  })
+
+  <p>In general, you may notice that ACL2 generates such ``special'' guard
+  conjectures for all calls of @('loop$') scions, whether or not they stemmed
+  from uses of @('loop$').  @('FROM/TO/BY') targets require that the bounds and
+  step all satisfy the @('of-type') specification, and the @('append') operator
+  requires that the loop body generate a @(tsee true-listp) (instead of an
+  @(tsee acl2-numberp) as required by the @('sum') operator.</p>
+
+  <h4>The Compromise Between Reasoning and Efficiency</h4>
+
+  <p>The translation of @('loop$') statements into formal terms reflects a
+  compromise between facilitating compositional reasoning and efficient
+  execution.</p>
+
+  <p>One sign of that compromise is our use of scions to handle @('until') and @('when')
+  clauses.  As noted above, by translating</p>
+
+  @({
+  (loop$ for x in lst until ... when ... collect ...)
+  })
+
+  <p>into</p>
+
+  @({
+  (collect$ ... (when$ ... (until$ ... lst)))
+  })
+
+  <p>we're forcing the evaluation of the formal semantics to copy the target
+  twice before collecting.  But it gives us the ability to reason
+  compositionally about @('collect$'), @('when$'), and @('until$').  We could
+  have defined a version of @('collect$') that took three @('lambda$')
+  expressions, one to terminate the collection, one to filter for the elements
+  we're interested in, and one to transform those elements into the values we
+  wish to collect.  This would avoid copying upon evaluation but make it more
+  difficult to reason.</p>
+
+  <p>Another example of compositionality is to consider a simple @('loop$')
+  over the @('in') target @('(append a b)').  There are 8 different ways you
+  can do a simple @('collect') over an @('(append a b)') target,</p>
+
+  @({
+  (loop$ for x in (append a b) collect (expr x))
+  (loop$ for x on (append a b) collect (expr x))
+  (loop$ for x in (append a b) until (stop x) collect (expr x))
+  (loop$ for x on (append a b) until (stop x) collect (expr x))
+  (loop$ for x in (append a b) when (test x) collect (expr x))
+  (loop$ for x on (append a b) when (test x) collect (expr x))
+  (loop$ for x in (append a b) until (stop x) when (test x)
+         collect (expr x))
+  (loop$ for x on (append a b) until (stop x) when (test x)
+         collect (expr x))
+  })
+
+  <p>Similarly, there are 8 ways to @('sum') over an @('(append a b)') target,
+  8 ways to @('append') over an @('(append a b)'), and 4 ways to @('always')
+  over an @('(append a b)') target.  Thus, there are 28 different simple
+  @('loop$')s over @('(append a b)').  And you can arrange to distribute the
+  @('loop$') over the @('(append a b)') with just six rewrite rules.</p>
+
+  @({
+  (equal (collect$ fn (append a b))
+         (append (collect$ fn a)
+                 (collect$ fn b)))
+
+  (equal (sum$ fn (append a b))
+         (+ (sum$ fn a)
+            (sum$ fn b)))
+
+  (equal (always$ fn (append a b))
+         (and (always$ fn a)
+              (always$ fn b)))
+
+  (equal (append$ fn (append a b))
+         (append (append$ fn a)
+                 (append$ fn b)))
+
+  (equal (until$ fn (append a b))
+         (if (exists$ fn a)
+             (until$ fn a)
+             (append a (until$ fn b))))
+
+  (equal (when$ fn (append a b))
+         (append (when$ fn a)
+                 (when$ fn b)))
+
+  })
+
+  <p>But to deal with fancy @('loop$') you need six more rewrite rules, one for
+  each fancy @('loop$') scion.  But every simple @('loop$') can be expressed by
+  an appropriate use of fancy scions.  We chose to break compositionality here
+  because we think simple @('loop$')s are most common and wanted to keep their
+  semantics simple.  I.e., we compromised.</p>
+
+  <p>By the way, if you want the prover to convert every simple scion to its
+  fancy counterpart you could prove rewrite rules like that below.</p>
+
+  @({
+  (defthm convert-collect$-to-collect$+
+    (implies (ok-fnp fn)
+             (equal (collect$ fn lst)
+                    (collect$+ `(lambda (loop$-gvars loop$-ivars)
+                                  (,fn (car loop$-ivars)))
+                               nil
+                               (loop$-as (list lst)))))
+    :hints ((\"[1]Goal\"
+             :expand ((tamep (cons fn '(x)))
+                      (tamep (cons fn '((car loop$-ivars))))))))
+  })")
 
 (defxdoc loop-stopper
   :parents (rewrite)
@@ -112434,7 +113097,8 @@ arithmetic) for libraries of @(see books) for arithmetic reasoning.</p>")
   @({
   '(LAMBDA (X)
            (DECLARE (TYPE (SATISFIES NATP) X)
-                    (XARGS :GUARD (NATP X) :SPLIT-TYPES T))
+                    (XARGS :GUARD (NATP X) :SPLIT-TYPES T)
+                    (IGNORABLE X))
            (RETURN-LAST 'PROGN
                         '(LAMBDA$ (X)
                                   (DECLARE (TYPE (SATISFIES NATP) X))
